<?xml version="1.0"?>
<rdf:RDF xmlns="http://sjka.site/ontology/atlas#"
     xml:base="http://sjka.site/ontology/atlas"
     xmlns:dc="http://purl.org/dc/elements/1.1/"
     xmlns:owl="http://www.w3.org/2002/07/owl#"
     xmlns:rdf="http://www.w3.org/1999/02/22-rdf-syntax-ns#"
     xmlns:xml="http://www.w3.org/XML/1998/namespace"
     xmlns:xsd="http://www.w3.org/2001/XMLSchema#"
     xmlns:prov="http://www.w3.org/ns/prov#"
     xmlns:rdfs="http://www.w3.org/2000/01/rdf-schema#"
     xmlns:atlas="http://sjka.site/ontology/atlas#"
     xmlns:terms="http://purl.org/dc/terms/">
    <owl:Ontology rdf:about="http://sjka.site/ontology/atlas#">
        <owl:imports rdf:resource="http://sjka.site/ontology/seips"/>
        <owl:imports rdf:resource="http://www.w3.org/ns/prov-o#"/>
        <dc:contributor xml:lang="en">Junli Liang</dc:contributor>
        <dc:contributor xml:lang="en">Rob Brennan</dc:contributor>
        <dc:creator xml:lang="en">Sajjad Karimian</dc:creator>
        <terms:created rdf:datatype="http://www.w3.org/2001/XMLSchema#date">2026-01-06</terms:created>
        <terms:description xml:lang="en">Atlas ontology for augmenting Socio-Technical Systems Analysis (STSA) with explicit, machine-readable data-flow and provenance modelling using PROV-O.</terms:description>
        <terms:license rdf:resource="https://creativecommons.org/licenses/by/4.0/"/>
        <terms:rights xml:lang="en">Copyright Â© 2025 Sajjad Karimian. Licensed under CC BY 4.0.</terms:rights>
        <terms:title xml:lang="en">Atlas Ontology</terms:title>
        <rdfs:label xml:lang="en">Atlas Ontology</rdfs:label>
        <owl:versionInfo>1.2</owl:versionInfo>
    </owl:Ontology>
    


    <!-- 
    ///////////////////////////////////////////////////////////////////////////////////////
    //
    // Annotation properties
    //
    ///////////////////////////////////////////////////////////////////////////////////////
     -->


    


    <!-- http://purl.org/dc/elements/1.1/contributor -->


    <owl:AnnotationProperty rdf:about="http://purl.org/dc/elements/1.1/contributor"/>
    


    <!-- http://purl.org/dc/elements/1.1/creator -->


    <owl:AnnotationProperty rdf:about="http://purl.org/dc/elements/1.1/creator"/>
    


    <!-- http://purl.org/dc/terms/created -->


    <owl:AnnotationProperty rdf:about="http://purl.org/dc/terms/created"/>
    


    <!-- http://purl.org/dc/terms/description -->


    <owl:AnnotationProperty rdf:about="http://purl.org/dc/terms/description"/>
    


    <!-- http://purl.org/dc/terms/license -->


    <owl:AnnotationProperty rdf:about="http://purl.org/dc/terms/license"/>
    


    <!-- http://purl.org/dc/terms/rights -->


    <owl:AnnotationProperty rdf:about="http://purl.org/dc/terms/rights"/>
    


    <!-- http://purl.org/dc/terms/title -->


    <owl:AnnotationProperty rdf:about="http://purl.org/dc/terms/title"/>
    


    <!-- http://sjka.site/ontology/atlas#hasCardinality -->


    <owl:AnnotationProperty rdf:about="http://sjka.site/ontology/atlas#hasCardinality">
        <rdfs:comment xml:lang="en">Used to describe whether a property is optional or mandatory for a class (documentation aid; not a logical constraint by itself).</rdfs:comment>
        <rdfs:label xml:lang="en">Cardinality Status</rdfs:label>
    </owl:AnnotationProperty>
    


    <!-- 
    ///////////////////////////////////////////////////////////////////////////////////////
    //
    // Datatypes
    //
    ///////////////////////////////////////////////////////////////////////////////////////
     -->


    


    <!-- http://www.w3.org/2001/XMLSchema#date -->


    <rdfs:Datatype rdf:about="http://www.w3.org/2001/XMLSchema#date"/>
    


    <!-- 
    ///////////////////////////////////////////////////////////////////////////////////////
    //
    // Object Properties
    //
    ///////////////////////////////////////////////////////////////////////////////////////
     -->


    


    <!-- http://sjka.site/ontology/atlas#playsRole -->


    <owl:ObjectProperty rdf:about="http://sjka.site/ontology/atlas#playsRole">
        <rdfs:domain rdf:resource="http://sjka.site/ontology/atlas#Actor"/>
        <rdfs:range rdf:resource="http://www.w3.org/ns/prov#Agent"/>
        <rdfs:comment xml:lang="en">Links an Actor to a role agent (e.g., DataProducer or DataConsumer) used for accountability modelling. Organisational responsibility can then be asserted using prov:actedOnBehalfOf from the role-agent to an Organisation.</rdfs:comment>
        <rdfs:label xml:lang="en">playsRole</rdfs:label>
    </owl:ObjectProperty>
    


    <!-- 
    ///////////////////////////////////////////////////////////////////////////////////////
    //
    // Classes
    //
    ///////////////////////////////////////////////////////////////////////////////////////
     -->


    


    <!-- http://sjka.site/ontology/atlas#Actor -->


    <owl:Class rdf:about="http://sjka.site/ontology/atlas#Actor">
        <rdfs:subClassOf rdf:resource="http://www.w3.org/ns/prov#Agent"/>
        <rdfs:subClassOf>
            <owl:Restriction>
                <owl:onProperty rdf:resource="http://sjka.site/ontology/atlas#playsRole"/>
                <owl:minCardinality rdf:datatype="http://www.w3.org/2001/XMLSchema#nonNegativeInteger">1</owl:minCardinality>
            </owl:Restriction>
        </rdfs:subClassOf>
        <hasCardinality xml:lang="en">mandatory</hasCardinality>
        <rdfs:comment xml:lang="en">Accountable actor performing or responsible for an activity (e.g., a microbiologist, IPC team member) in the provenance view.</rdfs:comment>
        <rdfs:label xml:lang="en">Actor</rdfs:label>
    </owl:Class>
    


    <!-- http://sjka.site/ontology/atlas#ContextualUse -->


    <owl:Class rdf:about="http://sjka.site/ontology/atlas#ContextualUse">
        <rdfs:subClassOf rdf:resource="http://www.w3.org/ns/prov#Activity"/>
        <hasCardinality xml:lang="en">mandatory</hasCardinality>
        <rdfs:comment xml:lang="en">Use of data in a specific context, role, and time (e.g., operational KPI computation and use).</rdfs:comment>
        <rdfs:label xml:lang="en">ContextualUse</rdfs:label>
    </owl:Class>
    


    <!-- http://sjka.site/ontology/atlas#DataConsumer -->


    <owl:Class rdf:about="http://sjka.site/ontology/atlas#DataConsumer">
        <rdfs:subClassOf rdf:resource="http://www.w3.org/ns/prov#Agent"/>
        <hasCardinality xml:lang="en">mandatory</hasCardinality>
        <rdfs:comment xml:lang="en">Role agent that consumes/uses data. Typically linked from an Actor via atlas:playsRole, and then linked to an Organisation via prov:actedOnBehalfOf.</rdfs:comment>
        <rdfs:label xml:lang="en">DataConsumer</rdfs:label>
    </owl:Class>
    


    <!-- http://sjka.site/ontology/atlas#DataFlow -->


    <owl:Class rdf:about="http://sjka.site/ontology/atlas#DataFlow">
        <rdfs:subClassOf rdf:resource="http://www.w3.org/ns/prov#Entity"/>
        <hasCardinality xml:lang="en">mandatory</hasCardinality>
        <rdfs:comment xml:lang="en">Data exchanged between components or activities (conceptual flow or exchanged dataset/transfer record).</rdfs:comment>
        <rdfs:label xml:lang="en">DataFlow</rdfs:label>
    </owl:Class>
    


    <!-- http://sjka.site/ontology/atlas#DataProcessing -->


    <owl:Class rdf:about="http://sjka.site/ontology/atlas#DataProcessing">
        <owl:equivalentClass rdf:resource="http://sjka.site/ontology/atlas#DataProcessingStep"/>
        <rdfs:subClassOf rdf:resource="http://www.w3.org/ns/prov#Activity"/>
        <hasCardinality xml:lang="en">mandatory</hasCardinality>
        <rdfs:comment xml:lang="en">Activity in which data are processed/transformed (e.g., extraction, cleaning, exporting, merging).</rdfs:comment>
        <rdfs:label xml:lang="en">DataProcessing</rdfs:label>
    </owl:Class>
    


    <!-- http://sjka.site/ontology/atlas#DataProcessingStep -->


    <owl:Class rdf:about="http://sjka.site/ontology/atlas#DataProcessingStep">
        <rdfs:subClassOf rdf:resource="http://www.w3.org/ns/prov#Activity"/>
        <rdfs:comment xml:lang="en">Deprecated in v1.2. Use atlas:DataProcessing (aligned with thesis schema, figure, and case study RDF).</rdfs:comment>
        <rdfs:label xml:lang="en">DataProcessingStep</rdfs:label>
        <owl:deprecated rdf:datatype="http://www.w3.org/2001/XMLSchema#boolean">true</owl:deprecated>
    </owl:Class>
    


    <!-- http://sjka.site/ontology/atlas#DataProducer -->


    <owl:Class rdf:about="http://sjka.site/ontology/atlas#DataProducer">
        <rdfs:subClassOf rdf:resource="http://www.w3.org/ns/prov#Agent"/>
        <hasCardinality xml:lang="en">mandatory</hasCardinality>
        <rdfs:comment xml:lang="en">Role agent that produces data. Typically linked from an Actor via atlas:playsRole, and then linked to an Organisation via prov:actedOnBehalfOf.</rdfs:comment>
        <rdfs:label xml:lang="en">DataProducer</rdfs:label>
    </owl:Class>
    


    <!-- http://sjka.site/ontology/atlas#DataStore -->


    <owl:Class rdf:about="http://sjka.site/ontology/atlas#DataStore">
        <rdfs:subClassOf rdf:resource="http://www.w3.org/ns/prov#Entity"/>
        <hasCardinality xml:lang="en">mandatory</hasCardinality>
        <rdfs:comment xml:lang="en">Location where data are stored (e.g., database, shared drive). Modelled as a PROV Entity to support prov:atLocation assertions.</rdfs:comment>
        <rdfs:label xml:lang="en">DataStore</rdfs:label>
    </owl:Class>
    


    <!-- http://sjka.site/ontology/atlas#DataValue -->


    <owl:Class rdf:about="http://sjka.site/ontology/atlas#DataValue">
        <rdfs:subClassOf rdf:resource="http://www.w3.org/ns/prov#Entity"/>
        <hasCardinality xml:lang="en">mandatory</hasCardinality>
        <rdfs:comment xml:lang="en">A data item/record/dataset used or produced in the workflow.</rdfs:comment>
        <rdfs:label xml:lang="en">DataValue</rdfs:label>
    </owl:Class>
    


    <!-- http://sjka.site/ontology/atlas#DerivedInsight -->


    <owl:Class rdf:about="http://sjka.site/ontology/atlas#DerivedInsight">
        <rdfs:subClassOf rdf:resource="http://www.w3.org/ns/prov#Entity"/>
        <hasCardinality xml:lang="en">mandatory</hasCardinality>
        <rdfs:comment xml:lang="en">An insight/metric/report derived from data values (e.g., a CPE report, KPIs).</rdfs:comment>
        <rdfs:label xml:lang="en">DerivedInsight</rdfs:label>
    </owl:Class>
    


    <!-- http://sjka.site/ontology/atlas#Environment -->


    <owl:Class rdf:about="http://sjka.site/ontology/atlas#Environment">
        <rdfs:subClassOf rdf:resource="http://sjka.site/ontology/seips#Environment"/>
        <hasCardinality xml:lang="en">optional</hasCardinality>
        <rdfs:comment xml:lang="en">Contextual environment aligned to the SEIPS work system model.</rdfs:comment>
        <rdfs:label xml:lang="en">Environment</rdfs:label>
    </owl:Class>
    


    <!-- http://sjka.site/ontology/atlas#ExternalEntity -->


    <owl:Class rdf:about="http://sjka.site/ontology/atlas#ExternalEntity">
        <rdfs:subClassOf rdf:resource="http://www.w3.org/ns/prov#Agent"/>
        <hasCardinality xml:lang="en">mandatory</hasCardinality>
        <rdfs:comment xml:lang="en">External agent involved in data operations (outside the focal organisational boundary).</rdfs:comment>
        <rdfs:label xml:lang="en">ExternalEntity</rdfs:label>
    </owl:Class>
    


    <!-- http://sjka.site/ontology/atlas#InternalEntity -->


    <owl:Class rdf:about="http://sjka.site/ontology/atlas#InternalEntity">
        <rdfs:subClassOf rdf:resource="http://www.w3.org/ns/prov#Agent"/>
        <hasCardinality xml:lang="en">mandatory</hasCardinality>
        <rdfs:comment xml:lang="en">Internal agent involved in data operations (inside the focal organisational boundary).</rdfs:comment>
        <rdfs:label xml:lang="en">InternalEntity</rdfs:label>
    </owl:Class>
    


    <!-- http://sjka.site/ontology/atlas#Interpretation -->


    <owl:Class rdf:about="http://sjka.site/ontology/atlas#Interpretation">
        <rdfs:subClassOf rdf:resource="http://www.w3.org/ns/prov#Activity"/>
        <hasCardinality xml:lang="en">mandatory</hasCardinality>
        <rdfs:comment xml:lang="en">Interpretation/analysis activity over data (e.g., interpreting an extract to produce a report).</rdfs:comment>
        <rdfs:label xml:lang="en">Interpretation</rdfs:label>
    </owl:Class>
    


    <!-- http://sjka.site/ontology/atlas#Organisation -->


    <owl:Class rdf:about="http://sjka.site/ontology/atlas#Organisation">
        <rdfs:subClassOf rdf:resource="http://www.w3.org/ns/prov#Agent"/>
        <hasCardinality xml:lang="en">optional</hasCardinality>
        <rdfs:comment xml:lang="en">Organisation responsible for data handling in the provenance view (modelled as a PROV Agent).</rdfs:comment>
        <rdfs:label xml:lang="en">Organisation</rdfs:label>
    </owl:Class>
    


    <!-- http://sjka.site/ontology/atlas#Process -->


    <owl:Class rdf:about="http://sjka.site/ontology/atlas#Process">
        <rdfs:subClassOf rdf:resource="http://www.w3.org/ns/prov#Activity"/>
        <hasCardinality xml:lang="en">mandatory</hasCardinality>
        <rdfs:comment xml:lang="en">A process step in which data operations are performed (high-level activity type used in Atlas).</rdfs:comment>
        <rdfs:label xml:lang="en">Process</rdfs:label>
    </owl:Class>
    


    <!-- http://sjka.site/ontology/atlas#SystemBoundary -->


    <owl:Class rdf:about="http://sjka.site/ontology/atlas#SystemBoundary">
        <rdfs:subClassOf rdf:resource="http://www.w3.org/ns/prov#Agent"/>
        <hasCardinality xml:lang="en">optional</hasCardinality>
        <rdfs:comment xml:lang="en">Represents the system boundary construct used to distinguish internal vs external agents/activities for governance and accountability. Modelled as an agent-like governance construct in the Atlas diagram.</rdfs:comment>
        <rdfs:label xml:lang="en">SystemBoundary</rdfs:label>
    </owl:Class>
    


    <!-- http://sjka.site/ontology/seips#Environment -->


    <owl:Class rdf:about="http://sjka.site/ontology/seips#Environment"/>
</rdf:RDF>



<!-- Generated by the OWL API (version 5.1.18) https://github.com/owlcs/owlapi/ -->


